#math 
[[Предел]]

$\exists \underset{x \rightarrow a}{\text{lim}}f(x) = L \in R \Leftrightarrow \exists L^-=\underset{x \rightarrow a-0}{\text{lim}}f(x), L^+=\underset{x \rightarrow a+0}{\text{lim}}f(x), L^-,L^+ \in R, L^+=L^-$
$\Rightarrow \underset{x \rightarrow a}{\text{lim}}f(x) = L \Leftrightarrow \forall \epsilon > 0 \exists \delta > 0 \forall x \in \stackrel{o}{U_{\delta}}(a) f(x)\in U_{\epsilon}(L)$
$\stackrel{o}{U_{\delta}(a) = (a - \delta; a) \cup (a;a+\delta)}$

$\underset{x \leftarrow a-0}{\text{lim}}f(x) = L^-: \forall \epsilon > 0\exists\delta>0 \forall x \in (a-\delta;a) f(x) \in U_{\epsilon}(L)$
$\underset{x \leftarrow a+0}{\text{lim}}f(x) = L^+: \forall \epsilon > 0\exists\delta>0 \forall x \in (a;a+\delta) f(x) \in U_{\epsilon}(L)$

$L^-=L^+=L$